Phi_Min_Lib.thy
@@ -11,6 +11,10 @@ section \<open>Preliminary\<close>
 
 declare Nat.One_nat_def[simp del] Num.add_2_eq_Suc'[simp del] split_paired_All[simp del]
 
+abbreviation LshR (infixl "LSHR" 70) where \<open>x LSHR y \<equiv> x div 2 ^ Big y\<close>
+abbreviation LshL (infixl "LSHL" 70) where \<open>x LSHL y \<equiv> x  *  2 ^ Big y\<close>
+
+definition Bits_Tag :: \<open>'a \<Rightarrow> nat \<Rightarrow> 'a\<close> (infix "<bits>" 25) where [iff]: \<open>(x <bits> n) = x\<close>
 
 section \<open>Basic Operations\<close>
 
@@ -102,7 +106,7 @@ proc op_set_var__synthesis[
 assumes G: \<open>\<^bold>p\<^bold>r\<^bold>o\<^bold>c g \<lbrace> X \<longmapsto> X1\<heavy_comma> SYNTHESIS \<^bold>v\<^bold>a\<^bold>l y \<Ztypecolon> U \<^bold>t\<^bold>h\<^bold>r\<^bold>o\<^bold>w\<^bold>s E\<rbrace> \<^bold>@\<^bold>G\<^bold>O\<^bold>A\<^bold>L G \<close>
   and S[unfolded Assertion_Level_Reasoning_def]:
         \<open>\<And>vy. PROP Assertion_Level_Reasoning(
-                  \<^bold>v\<^bold>i\<^bold>e\<^bold>w X1\<heavy_comma> y \<Ztypecolon> Val vy U \<longmapsto> \<blangle> Y\<heavy_comma> x \<Ztypecolon> Var var T\<heavy_comma> y \<Ztypecolon> Val vy U \<brangle> \<^bold>w\<^bold>i\<^bold>t\<^bold>h Any)\<close>
+                  \<^bold>v\<^bold>i\<^bold>e\<^bold>w X1\<heavy_comma> y \<Ztypecolon> Val vy U \<longmapsto> Y\<heavy_comma> x \<Ztypecolon> Var var T\<heavy_comma> y \<Ztypecolon> Val vy U \<^bold>w\<^bold>i\<^bold>t\<^bold>h Any)\<close>
   and [\<phi>reason on \<open>\<phi>SemType (x \<Ztypecolon> T) ?TY\<close>]: \<open>\<phi>SemType (x \<Ztypecolon> T) TY\<close>
   and [\<phi>reason on \<open>\<phi>SemType (y \<Ztypecolon> U) ?TY\<close>]: \<open>\<phi>SemType (y \<Ztypecolon> U) TY\<close>
  goal G
@@ -241,7 +245,18 @@ lemma [\<phi>reason 1200
   for X :: \<open>'ret \<Rightarrow> ('FIC_N,'FIC) assn\<close>
   unfolding Synthesis_Parse_def ..
 
-lemma [\<phi>reason
+lemma [\<phi>reason 1200
+    on \<open>PROP Synthesis_Parse ((numeral ?n::nat) <bits> ?b) (?X :: ?'ret \<Rightarrow> ('FIC_N,'FIC) assn)\<close>
+       \<open>PROP Synthesis_Parse ((1::nat) <bits> ?b) (?X :: ?'ret \<Rightarrow> ('FIC_N,'FIC) assn)\<close>
+       \<open>PROP Synthesis_Parse ((0::nat) <bits> ?b) (?X :: ?'ret \<Rightarrow> ('FIC_N,'FIC) assn)\<close>
+]:
+  \<open> PROP Synthesis_Parse (n \<Ztypecolon> \<nat>[b]) X
+\<Longrightarrow> PROP Synthesis_Parse (n <bits> b) X\<close>
+  for X :: \<open>'ret \<Rightarrow> ('FIC_N,'FIC) assn\<close>
+  unfolding Synthesis_Parse_def ..
+
+
+lemma [\<phi>reason 1200
     on \<open>\<^bold>p\<^bold>r\<^bold>o\<^bold>c ?f \<lbrace> ?X' \<longmapsto> ?X\<heavy_comma> SYNTHESIS \<^bold>v\<^bold>a\<^bold>l numeral ?n \<Ztypecolon> \<nat>[?b] \<^bold>t\<^bold>h\<^bold>r\<^bold>o\<^bold>w\<^bold>s ?E \<rbrace> \<^bold>@\<^bold>G\<^bold>O\<^bold>A\<^bold>L ?G\<close>
        \<open>\<^bold>p\<^bold>r\<^bold>o\<^bold>c ?f \<lbrace> ?X' \<longmapsto> ?X\<heavy_comma> SYNTHESIS \<^bold>v\<^bold>a\<^bold>l 1 \<Ztypecolon> \<nat>[?b] \<^bold>t\<^bold>h\<^bold>r\<^bold>o\<^bold>w\<^bold>s ?E \<rbrace> \<^bold>@\<^bold>G\<^bold>O\<^bold>A\<^bold>L ?G\<close>
        \<open>\<^bold>p\<^bold>r\<^bold>o\<^bold>c ?f \<lbrace> ?X' \<longmapsto> ?X\<heavy_comma> SYNTHESIS \<^bold>v\<^bold>a\<^bold>l 0 \<Ztypecolon> \<nat>[?b] \<^bold>t\<^bold>h\<^bold>r\<^bold>o\<^bold>w\<^bold>s ?E \<rbrace> \<^bold>@\<^bold>G\<^bold>O\<^bold>A\<^bold>L ?G\<close>
@@ -250,6 +265,15 @@ lemma [\<phi>reason
 \<Longrightarrow> \<^bold>p\<^bold>r\<^bold>o\<^bold>c op_const_int b n \<lbrace> R \<longmapsto> R\<heavy_comma> SYNTHESIS \<^bold>v\<^bold>a\<^bold>l n \<Ztypecolon> \<nat>[b] \<rbrace> \<^bold>@\<^bold>G\<^bold>O\<^bold>A\<^bold>L G\<close>
   unfolding Synthesis_def GOAL_CTXT_def
   using op_const_int_\<phi>app[THEN \<phi>frame, simplified] .
+
+
+lemma [\<phi>reason 1200
+    on \<open>\<^bold>p\<^bold>r\<^bold>o\<^bold>c ?f \<lbrace> ?R \<longmapsto> ?R' \<heavy_comma> SYNTHESIS \<^bold>v\<^bold>a\<^bold>l (?n <bits> ?b') \<Ztypecolon> \<nat>[?b] \<^bold>t\<^bold>h\<^bold>r\<^bold>o\<^bold>w\<^bold>s ?E \<rbrace> \<^bold>@\<^bold>G\<^bold>O\<^bold>A\<^bold>L ?G\<close>
+]:
+  \<open> \<^bold>p\<^bold>r\<^bold>o\<^bold>c f \<lbrace> R \<longmapsto> R' \<heavy_comma> SYNTHESIS \<^bold>v\<^bold>a\<^bold>l n \<Ztypecolon> \<nat>[b] \<^bold>t\<^bold>h\<^bold>r\<^bold>o\<^bold>w\<^bold>s E \<rbrace> \<^bold>@\<^bold>G\<^bold>O\<^bold>A\<^bold>L G
+\<Longrightarrow> \<^bold>p\<^bold>r\<^bold>o\<^bold>c f \<lbrace> R \<longmapsto> R' \<heavy_comma> SYNTHESIS \<^bold>v\<^bold>a\<^bold>l (n <bits> b) \<Ztypecolon> \<nat>[b] \<^bold>t\<^bold>h\<^bold>r\<^bold>o\<^bold>w\<^bold>s E \<rbrace> \<^bold>@\<^bold>G\<^bold>O\<^bold>A\<^bold>L G\<close>
+  unfolding Bits_Tag_def .
+
 
 lemma op_const_size_t:
   \<open>\<^bold>p\<^bold>r\<^bold>o\<^bold>c op_const_size_t n \<lbrace> Void \<longmapsto> \<^bold>v\<^bold>a\<^bold>l n \<Ztypecolon> Size \<rbrace>\<close>
@@ -354,6 +378,43 @@ proc [
   throws \<open>E1 + E2\<close>
   \<medium_left_bracket> F1 F2 / \<medium_right_bracket>. .
 
+paragraph \<open>Shift\<close>
+
+lemma op_lshr_nat_\<phi>app:
+  \<open>\<^bold>p\<^bold>r\<^bold>o\<^bold>c op_lshr b1 b2 (\<phi>V_pair raw2 raw1) \<lbrace> x \<Ztypecolon> Val raw1 \<nat>[b1] \<heavy_comma> y \<Ztypecolon> Val raw2 \<nat>[b2] \<longmapsto> \<^bold>v\<^bold>a\<^bold>l x div 2 ^ Big y \<Ztypecolon> \<nat>[b1] \<rbrace>\<close>
+  unfolding op_lshr_def
+  apply (cases raw1; cases raw2; simp; \<phi>reason; simp add: \<phi>expns Big_def)
+  using div_le_dividend le_less_trans by blast
+
+lemma op_lshl_nat_\<phi>app:
+  \<open> \<^bold>p\<^bold>r\<^bold>e\<^bold>m\<^bold>i\<^bold>s\<^bold>e x * 2 ^ Big y < 2 ^ Big b1
+\<Longrightarrow> \<^bold>p\<^bold>r\<^bold>o\<^bold>c op_lshl b1 b2 (\<phi>V_pair raw2 raw1) \<lbrace> x \<Ztypecolon> Val raw1 \<nat>[b1] \<heavy_comma> y \<Ztypecolon> Val raw2 \<nat>[b2] \<longmapsto> \<^bold>v\<^bold>a\<^bold>l x * 2 ^ Big y \<Ztypecolon> \<nat>[b1] \<rbrace>\<close>
+  unfolding op_lshl_def
+  by (cases raw1; cases raw2; simp; \<phi>reason; simp add: \<phi>expns Big_def)
+
+proc [
+    \<phi>reason 1300 on \<open>\<^bold>p\<^bold>r\<^bold>o\<^bold>c ?F \<lbrace> ?R \<longmapsto> \<lambda>ret. ?R2\<heavy_comma> SYNTHESIS (?x LSHR ?y) \<Ztypecolon> ?T ret \<^bold>t\<^bold>h\<^bold>r\<^bold>o\<^bold>w\<^bold>s ?E \<rbrace> \<^bold>@\<^bold>G\<^bold>O\<^bold>A\<^bold>L ?G\<close>
+]:
+  assumes F1: \<open>\<^bold>p\<^bold>r\<^bold>o\<^bold>c f1 \<lbrace> R  \<longmapsto> R1\<heavy_comma> SYNTHESIS \<^bold>v\<^bold>a\<^bold>l x \<Ztypecolon> \<nat>[b1] \<^bold>t\<^bold>h\<^bold>r\<^bold>o\<^bold>w\<^bold>s E1 \<rbrace>  \<^bold>@\<^bold>G\<^bold>O\<^bold>A\<^bold>L G\<close>
+    and   F2: \<open>\<^bold>p\<^bold>r\<^bold>o\<^bold>c f2 \<lbrace> R1 \<longmapsto> R2\<heavy_comma> SYNTHESIS \<^bold>v\<^bold>a\<^bold>l y \<Ztypecolon> \<nat>[b2] \<^bold>t\<^bold>h\<^bold>r\<^bold>o\<^bold>w\<^bold>s E2 \<rbrace>  \<^bold>@\<^bold>G\<^bold>O\<^bold>A\<^bold>L G\<close>
+  goal G
+  argument \<open>R\<close>
+  return   \<open>R2\<heavy_comma> SYNTHESIS \<^bold>v\<^bold>a\<^bold>l (x LSHR y) \<Ztypecolon> \<nat>[b1]\<close>
+  throws \<open>E1 + E2\<close>
+  \<medium_left_bracket> F1 F2 op_lshr_nat \<medium_right_bracket>. .
+
+proc [
+    \<phi>reason 1300 on \<open>\<^bold>p\<^bold>r\<^bold>o\<^bold>c ?F \<lbrace> ?R \<longmapsto> \<lambda>ret. ?R2\<heavy_comma> SYNTHESIS (?x LSHL ?y) \<Ztypecolon> ?T ret \<^bold>t\<^bold>h\<^bold>r\<^bold>o\<^bold>w\<^bold>s ?E \<rbrace> \<^bold>@\<^bold>G\<^bold>O\<^bold>A\<^bold>L ?G\<close>
+]:
+  premises \<open>x * 2 ^ Big y < 2 ^ Big b1\<close>
+  assumes F1: \<open>\<^bold>p\<^bold>r\<^bold>o\<^bold>c f1 \<lbrace> R  \<longmapsto> R1\<heavy_comma> SYNTHESIS \<^bold>v\<^bold>a\<^bold>l x \<Ztypecolon> \<nat>[b1] \<^bold>t\<^bold>h\<^bold>r\<^bold>o\<^bold>w\<^bold>s E1 \<rbrace>  \<^bold>@\<^bold>G\<^bold>O\<^bold>A\<^bold>L G\<close>
+    and   F2: \<open>\<^bold>p\<^bold>r\<^bold>o\<^bold>c f2 \<lbrace> R1 \<longmapsto> R2\<heavy_comma> SYNTHESIS \<^bold>v\<^bold>a\<^bold>l y \<Ztypecolon> \<nat>[b2] \<^bold>t\<^bold>h\<^bold>r\<^bold>o\<^bold>w\<^bold>s E2 \<rbrace>  \<^bold>@\<^bold>G\<^bold>O\<^bold>A\<^bold>L G\<close>
+  goal G
+  argument \<open>R\<close>
+  return   \<open>R2\<heavy_comma> SYNTHESIS \<^bold>v\<^bold>a\<^bold>l (x LSHL y) \<Ztypecolon> \<nat>[b1]\<close>
+  throws \<open>E1 + E2\<close>
+  \<medium_left_bracket> F1 F2 op_lshl_nat \<medium_right_bracket>. .
+
 
 paragraph \<open>Less Than\<close>
 
@@ -372,9 +433,7 @@ proc [
   argument \<open>R\<close>
   return   \<open>R2\<heavy_comma> SYNTHESIS \<^bold>v\<^bold>a\<^bold>l (x < y) \<Ztypecolon> \<bool>\<close>
   throws \<open>E1 + E2\<close>
-  \<medium_left_bracket>
-  ;; F1
-  ;; F2 < \<medium_right_bracket>. .
+  \<medium_left_bracket> F1 F2 < \<medium_right_bracket>. .
 
 proc [
     \<phi>reason on \<open>\<^bold>p\<^bold>r\<^bold>o\<^bold>c ?F \<lbrace> ?R \<longmapsto> \<lambda>ret. ?R2\<heavy_comma> SYNTHESIS (?x > ?y) \<Ztypecolon> ?T ret \<^bold>t\<^bold>h\<^bold>r\<^bold>o\<^bold>w\<^bold>s ?E \<rbrace> \<^bold>@\<^bold>G\<^bold>O\<^bold>A\<^bold>L ?G\<close>
